src/Idempotent.v
@@ -1,60 +1,25 @@
-Require Import Hoare.
+Require Import Mem Hoare.
 Require Import Prog ProgMonad.
 Require Import Pred PredCrash.
 Require Import SepAuto.
 Require Import AsyncDisk.
 Require Import Hashmap.
 
-
-Lemma hashmap_subset_some_list_trans : forall hm hm' hm'',
-    (exists l, hashmap_subset l hm hm') ->
-    (exists l, hashmap_subset l hm' hm'') ->
-    exists l, hashmap_subset l hm hm''.
-Proof.
-  intros; solve_hashmap_subset.
-Qed.
-
 Lemma finished_val_eq : forall T d dm bm (v:T),
     exists v', Finished d bm dm v = Finished d bm dm v'.
 Proof. eauto. Qed.
 
 Hint Resolve finished_val_eq.
-(*
-Lemma exec_crashed_hashmap_subset' : forall T (p: prog T) d dt d' dt' bm bt bm' bt' out tr pr,
-  exec pr d dt bm bt p out tr
-  -> (out = Crashed d' dt' bm' bt' \/ exists v, out = Finished d' dt' bm' bt' v)
-  -> exists l, hashmap_subset l hm hm'.
-Proof.
-  intros.
-  generalize dependent bm'.
-  generalize dependent hm'.
-  generalize dependent m'.
-  
-  
-    induction H; subst; try solve [ intuition; repeat deex; try congruence;
-    try match goal with
-        | [ H: @eq (result) _ _ |- _ ] =>
-          inversion H; subst
-        end;
-    eauto; solve_hashmap_subset].
 
-    intros.
-    split_ors.    
-    eauto 10 using hashmap_subset_some_list_trans.
-    eauto 7 using hashmap_subset_some_list_trans.
-Qed.
- *)
 
-(*
-Lemma exec_crashed_blockmem_subset' : forall T (p: prog T) d dt d' dt' bm bt bm' bt' out tr pr,
+Lemma exec_crashed_blockmem_subset' : forall T (p: prog T) d dm d' dm' bm bm' out tr pr,
   exec pr d bm dm p out tr
   -> (out = Crashed d' bm' dm' \/ exists v, out = Finished d' bm' dm' v)
   -> bm c= bm'.
 Proof.
   intros.
   generalize dependent bm'.
-  generalize dependent bt'.
-  generalize dependent dt'.
+  generalize dependent dm'.
   generalize dependent d'.
   
   
@@ -67,92 +32,53 @@ Proof.
 
     intros.
     split_ors.    
-    eauto 10 using hashmap_subset_some_list_trans.
-    eauto 7 using hashmap_subset_some_list_trans.
+    eauto 10.
+    eauto 7.
 Qed.
-*)
-(*
-Lemma exec_crashed_hashmap_subset : forall T (p: prog T) pr tr m m' bm hm bm' hm' out,
-  exec pr m bm hm p out tr
-  -> out = Crashed  m' bm' hm'
-  -> exists l, hashmap_subset l hm hm'.
-Proof.
-  intros.
-  eapply exec_crashed_hashmap_subset'; eauto.
-Qed.
- *)
-(*
-Lemma exec_crashed_blockmem_subset : forall T (p: prog T) d dt d' dt' bm bt bm' bt' out tr pr,
-  exec pr d dt bm bt p out tr
-  -> out = Crashed d' dt' bm' bt'
+
+Lemma exec_crashed_blockmem_subset : forall T (p: prog T) d dm d' dm' bm bm' out tr pr,
+  exec pr d bm dm p out tr
+  -> out = Crashed d' bm' dm'
   -> bm c= bm'.
 Proof.
   intros.
   eapply exec_crashed_blockmem_subset'; eauto.
 Qed.
-*)
-(*
-Ltac solve_hashmap_subset' :=
-  match goal with
-  | [ H: exec _ _ _ _ (Crashed _ _ _), Hpre: forall (_ : hashmap), _ =p=> ?pre _ _ _
-      |- forall (_ : hashmap), _ =p=> ?pre _ _ _ ]
-    => eapply exec_crashed_hashmap_subset in H as H'; eauto;
-        intros;
-        eapply pimpl_trans; try apply Hpre;
-        autorewrite with crash_xform; cancel
-  | [ |- context[hashmap_subset] ]
-        => pred_apply; cancel
-  end; try solve [
-    repeat match goal with
-    | [ H: forall (_ : hashmap), _ =p=> _ |- _ ] => clear H
-    end; solve_hashmap_subset
-  ].
- *)
-(*
+
 Lemma corr3_from_corr2_failed:
   forall (TF TR: Type) pr tr m mr bmr hmr (p: prog TF) (r: prog TR) out
-         (crash: block_mem -> hashmap -> pred) ppre rpre crashdone_p crashdone_r,
-  exec_recover pr mr bmr hmr p r out tr
+         (crash: taggedmem -> domainmem -> pred) ppre rpre crashdone_p crashdone_r,
+  exec_recover pr mr empty_mem empty_mem p r out tr
   -> TF = TR
   -> possible_crash m mr
   -> crash bmr hmr m
-  -> (forall bm' hm', crash_xform (crash bm' hm'
-     * [[ exists l, hashmap_subset l hmr hm' ]] *
-     [[ bmr c= bm' ]])
-      =p=> ppre crashdone_p crash bm' hm')
-  -> (forall bm' hm', crash_xform (crash bm' hm'
-      * [[ exists l, hashmap_subset l hmr hm' ]] *
-     [[ bmr c= bm' ]])
-      =p=> rpre crashdone_r crash bm' hm')
+  -> (forall bm' hm', crash_xform (crash bm' hm')
+      =p=> ppre crashdone_p crash empty_mem empty_mem)
+  -> (forall bm' hm', crash_xform (crash bm' hm')
+      =p=> rpre crashdone_r crash empty_mem empty_mem)
   -> {{ pr | ppre }} p
   -> {{ pr | rpre }} r
-  -> forall mx bmx hmx, out <> RFailed TF TR mx bmx hmx.
+  -> out <> RFailed TF TR.
 Proof.
   intros.
   generalize dependent m.
   induction H; intros; try congruence.
   - edestruct H5; eauto.
     eapply H3. eapply crash_xform_apply; eauto.
-    pred_apply; cancel.
-    solve_hashmap_subset.
     repeat (destruct H7; try congruence).
 Qed.
 
 Lemma corr3_from_corr2_finished:
   forall (TF TR: Type) pr tr m mr bmr hmr (p: prog TF) (r: prog TR) out
-    (crash: block_mem -> hashmap -> pred) ppre rpre crashdone_p crashdone_r m' bm' hm' v,
-  exec_recover pr mr bmr hmr p r out tr
+    (crash: taggedmem -> domainmem -> pred) ppre rpre crashdone_p crashdone_r m' bm' hm' v,
+  exec_recover pr mr empty_mem empty_mem p r out tr
   -> TF = TR
   -> possible_crash m mr
   -> crash bmr hmr m
-  -> (forall bm' hm', crash_xform (crash bm' hm'
-     * [[ exists l, hashmap_subset l hmr hm' ]] *
-     [[ bmr c= bm' ]])
-      =p=> ppre crashdone_p crash bm' hm')
-  -> (forall bm' hm', crash_xform (crash bm' hm'
-      * [[ exists l, hashmap_subset l hmr hm' ]] *
-     [[ bmr c= bm' ]])
-      =p=> rpre crashdone_r crash bm' hm')
+  -> (forall bm' hm', crash_xform (crash bm' hm')
+      =p=> ppre crashdone_p crash empty_mem empty_mem)
+  -> (forall bm' hm', crash_xform (crash bm' hm')
+      =p=> rpre crashdone_r crash empty_mem empty_mem)
   -> {{ pr | ppre }} p
   -> {{ pr | rpre }} r
   -> out = RFinished TR m' bm' hm' v
@@ -162,28 +88,23 @@ Proof.
   induction H; try congruence.
   edestruct H5; eauto.
   - eapply H3. eapply crash_xform_apply; eauto.
-    pred_apply; cancel.
-    solve_hashmap_subset.
   - split_ors; cleanup; try congruence; split; eauto; congruence.
 Qed.
 
+
 Lemma corr3_from_corr2_recovered:
-  forall (TF TR: Type) mr bmr hmr (p: prog TF) (r: prog TR) out
-         (crash: block_mem -> hashmap -> pred) ppre rpre crashdone_p crashdone_r m' bm' hm' v pr tr,
-  exec_recover pr mr bmr hmr p r out tr
+  forall (TF TR: Type) mr (p: prog TF) (r: prog TR) out bm hm
+         (crash: taggedmem -> domainmem -> pred) ppre rpre crashdone_p crashdone_r m' bm' hm' v pr tr,
+  exec_recover pr mr bm hm p r out tr
   -> out = RRecovered TF m' bm' hm' v  
   -> TF = TR
-  -> forall m,
+  -> forall m bmr hmr,
     possible_crash m mr
   -> crash bmr hmr m
-  -> (forall bm' hm', crash_xform (crash bm' hm'
-     * [[ exists l, hashmap_subset l hmr hm' ]] *
-     [[ bmr c= bm' ]])
-      =p=> ppre crashdone_p crash bm' hm')
-  -> (forall bm' hm', crash_xform (crash bm' hm'
-     * [[ exists l, hashmap_subset l hmr hm' ]]
-     * [[ bmr c= bm' ]])
-      =p=> rpre crashdone_r crash bm' hm')
+  -> (forall bm' hm', crash_xform (crash bm' hm')
+      =p=> ppre crashdone_p crash bm hm)
+  -> (forall bm' hm', crash_xform (crash bm' hm')
+      =p=> rpre crashdone_r crash empty_mem empty_mem)
   -> {{ pr | ppre }} p
   -> {{ pr | rpre }} r
   -> crashdone_r m' bm' hm' v /\ only_public_operations tr.
@@ -192,16 +113,11 @@ Proof.
   - inversion H2; subst; clear H2.
     edestruct H8; eauto.
     eapply H6; eapply crash_xform_apply; eauto.
-    pred_apply; cancel.
-    solve_hashmap_subset.
     split_ors; cleanup; try congruence.
     inversion H1; subst.
     edestruct H9; eauto.
     
     eapply H7; eapply crash_xform_apply; eauto.
-    pred_apply; cancel.
-    eapply exec_crashed_hashmap_subset; eauto.
-    eapply exec_crashed_blockmem_subset; eauto.
     split_ors; cleanup; try congruence.
     split; eauto.
     apply only_public_operations_app_merge; eauto.
@@ -209,49 +125,10 @@ Proof.
   - inversion H2; subst; clear H2.
     edestruct H8; eauto.
     eapply H6; eapply crash_xform_apply; eauto.
-    pred_apply; cancel.
-    solve_hashmap_subset.
     split_ors; cleanup; try congruence.
     edestruct IHexec_recover; eauto.
-
-    intros.
-    repeat rewrite crash_xform_sep_star_dist.
-    xcrash.
-    rewrite <- H7; cancel.
-    rewrite crash_xform_sep_star_dist.
-    cancel.
-    repeat rewrite crash_xform_lift_empty; cancel.
-    rewrite crash_xform_sep_star_dist.
-    cancel.
-    repeat rewrite crash_xform_lift_empty; cancel.
-    eapply hashmap_subset_some_list_trans; eauto.
-    eapply exec_crashed_hashmap_subset; eauto.
-    intros _ _.
-    eapply block_mem_subset_trans.
-    eapply exec_crashed_blockmem_subset; eauto.
-    eauto.
-
-    intros.
-    repeat rewrite crash_xform_sep_star_dist.
-    xcrash.
-    rewrite <- H7; cancel.
-    rewrite crash_xform_sep_star_dist.
-    cancel.
-    repeat rewrite crash_xform_lift_empty; cancel.
-    rewrite crash_xform_sep_star_dist.
-    cancel.
-    repeat rewrite crash_xform_lift_empty; cancel.
-    eapply hashmap_subset_some_list_trans; eauto.
-    eapply exec_crashed_hashmap_subset; eauto.
-    intros _ _.
-    eapply block_mem_subset_trans.
-    eapply exec_crashed_blockmem_subset; eauto.
-    eauto.
-    
     split; eauto.
     apply only_public_operations_app_merge; eauto.
-    Unshelve.
-    all: unfold Mem.EqDec; apply handle_eq_dec.
 Qed.
 
 Theorem corr3_from_corr2:
@@ -261,10 +138,8 @@ Theorem corr3_from_corr2:
   -> {{ pr | fun bm hm done crashdone => exists crash,
         ppre done crash bm hm
         * [[ forall bm' hm',
-          crash_xform (crash bm' hm'
-          * [[ exists l, hashmap_subset l hm hm' ]]
-          * [[ bm c= bm' ]])
-          =p=> rpre crashdone crash bm' hm' ]] }} p >> r.
+          crash_xform (crash bm' hm')
+          =p=> rpre crashdone crash empty_mem empty_mem ]] }} p >> r.
 Proof.
   unfold corr3; intros.
   destruct H1 as [crash H1].
@@ -284,10 +159,6 @@ Proof.
     edestruct H0; eauto.
     eapply H5.
     eapply crash_xform_apply; eauto.
-    pred_apply; cancel.
-    eauto.
-    eapply exec_crashed_hashmap_subset; eauto.
-    eapply exec_crashed_blockmem_subset; eauto.
     split_ors; cleanup; try congruence.
     split.
     right; repeat eexists; eauto.
@@ -300,47 +171,11 @@ Proof.
     apply H6.
     all: eauto.
 
-    intros.
-    repeat rewrite crash_xform_sep_star_dist.
-    xcrash.
-    rewrite <- H5; cancel.
-    rewrite crash_xform_sep_star_dist.
-    cancel.
-    repeat rewrite crash_xform_lift_empty; cancel.
-    rewrite crash_xform_sep_star_dist.
-    cancel.
-    repeat rewrite crash_xform_lift_empty; cancel.
-    eapply hashmap_subset_some_list_trans; eauto.
-    eapply exec_crashed_hashmap_subset; eauto.
-    intros _ _.
-    eapply block_mem_subset_trans.
-    eapply exec_crashed_blockmem_subset; eauto.
-    eauto.
-
-    intros.
-    repeat rewrite crash_xform_sep_star_dist.
-    xcrash.
-    rewrite <- H5; cancel.
-    rewrite crash_xform_sep_star_dist.
-    cancel.
-    repeat rewrite crash_xform_lift_empty; cancel.
-    rewrite crash_xform_sep_star_dist.
-    cancel.
-    repeat rewrite crash_xform_lift_empty; cancel.
-    eapply hashmap_subset_some_list_trans; eauto.
-    eapply exec_crashed_hashmap_subset; eauto.
-    intros _ _.
-    eapply block_mem_subset_trans.
-    eapply exec_crashed_blockmem_subset; eauto.
-    eauto.
-    
     split; eauto.
     right; repeat eexists; eauto.
     apply only_public_operations_app_merge; eauto.
-
-    Unshelve.
-    all: unfold Mem.EqDec; apply handle_eq_dec.
 Qed.
+
 
 Theorem corr3_from_corr2_rx :
   forall TF TR RF RR pr (p: prog TF) (r:  prog TR)
@@ -351,10 +186,8 @@ Theorem corr3_from_corr2_rx :
   -> {{ pr | fun bm hm done crashdone => exists crash,
         ppre done crash bm hm        
         * [[ forall bm' hm',
-          crash_xform (crash bm' hm'
-          * [[ exists l, hashmap_subset l hm hm' ]]
-          * [[ bm c= bm' ]])
-          =p=> rpre crashdone crash bm' hm']] }} Bind p rxp >> Bind r rxr.
+          crash_xform (crash bm' hm')
+          =p=> rpre crashdone crash empty_mem empty_mem]] }} Bind p rxp >> Bind r rxr.
 Proof.
   intros.
   apply corr3_from_corr2; eauto.
@@ -370,4 +203,3 @@ Qed.
       | [ H: diskIs _ _ |- _ ] => unfold diskIs in *
       | [ |- pimpl (crash_xform _) _ ] => progress autorewrite with crash_xform
     end.
-*)
